src/spec/core/TLS13.Wire.Spec.fsti
@@ -24,6 +24,7 @@ module GESG = TLS13.Wire.Generated.ExtensionClientHello_extension_data_supported
 module GHS = TLS13.Wire.Generated.Handshake
 module GNG = TLS13.Wire.Generated.NamedGroup
 module GPV = TLS13.Wire.Generated.ProtocolVersion
+module GOV = TLS13.Wire.Generated.OfferedVersion
 module GSH = TLS13.Wire.Generated.ServerHello
 module GSHB = TLS13.Wire.Generated.ServerHello_body
 module GSHBody = TLS13.Wire.Generated.ServerHelloBody
@@ -277,7 +278,7 @@ val lemma_ch_extensions_cons_sv:
   sv:bool ->
   ss:list T.signature_scheme ->
   Lemma (ch_extensions (GECH.Extension_data_supported_versions svl :: tl) sn ks sv ss ==
-         (if FStar.List.Tot.mem GPV.TLS_1p3 svl
+         (if FStar.List.Tot.mem GOV.Offered_TLS_1p3 svl
           then ch_extensions tl sn ks true ss
           else None))
 
